policy_proof/coq/prov.v
@@ -1,0 +1,29 @@
+Require Import Coq.Lists.List.
+Require Import Unicode.Utf8.
+
+Require Import types.
+Require Import data_model.
+
+Inductive prov_type: Set :=
+  | prov_trans: simple_transform_func -> prov_type
+  | prov_agg: simple_aggregate_func -> prov_type
+  | prov_noise: prov_type
+.
+
+Definition prov_type_label (pt: prov_type): (Policy.policy * Policy.policy) :=
+  match pt with
+  | prov_trans _ => (Policy.policy_transform, Policy.policy_agg)
+  | prov_agg _ => (Policy.policy_transform, Policy.policy_agg)
+  | prov_noise => (Policy.policy_agg, Policy.policy_noise)
+  end.
+
+(*
+    This is an auxiliary definition to help us define the prov type to help prove the
+    main theorem that involve the "flow" of each sensitive data piece at the cell level.
+*)
+Inductive prov: Set :=
+  | prov_list: prov_type -> list (nat * prov) -> prov
+  | prov_none: prov
+.
+
+Definition prov_ctx := list (nat * prov).
